validate vldata

src/lowparse/LowParse.Low.VLData.fst
@@ -4,74 +4,67 @@ include LowParse.Low.FLData
 
 module B = LowStar.Buffer
 module HST = FStar.HyperStack.ST
+module U32 = FStar.UInt32
 
 inline_for_extraction
-let parse32_bounded_integer
+let read_bounded_integer
   (i: integer_size)
-: Tot (parser32 (parse_bounded_integer i))
+: Tot (leaf_reader (parse_bounded_integer i))
 = [@inline_let]
   let _ = integer_size_values i in
   match i with
-  | 1 -> parse32_bounded_integer_1 ()
-  | 2 -> parse32_bounded_integer_2 ()
-  | 3 -> parse32_bounded_integer_3 ()
-  | 4 -> parse32_bounded_integer_4 ()
-
-module I32 = FStar.Int32
+  | 1 -> read_bounded_integer_1 ()
+  | 2 -> read_bounded_integer_2 ()
+  | 3 -> read_bounded_integer_3 ()
+  | 4 -> read_bounded_integer_4 ()
 
 inline_for_extraction
-let validate32_bounded_integer
+let validate_bounded_integer
+  [| validator_cls |]
   (i: integer_size)
-  (i32: I32.t { I32.v i32 == i } )
-: Tot (validator32 (parse_bounded_integer i))
-= validate32_total_constant_size (parse_bounded_integer i) i32 ()
-
-module U32 = FStar.UInt32
-module Cast = FStar.Int.Cast
+  (i32: U32.t { U32.v i32 == i } )
+: Tot (validator (parse_bounded_integer i))
+= validate_total_constant_size (parse_bounded_integer i) i32 ()
 
 inline_for_extraction
-let validate32_vldata_payload
+let validate_vldata_payload
+  [| validator_cls |]
   (sz: integer_size)
   (f: ((x: bounded_integer sz) -> GTot bool))
-  (f_lemma: ((x: bounded_integer sz) -> Lemma (f x == true ==> U32.v x < 2147483648)))
   (#k: parser_kind)
   (#t: Type0)
   (#p: parser k t)
-  (v: validator32 p)
+  (v: validator p)
   (i: bounded_integer sz { f i == true } )
-: Tot (validator32 (parse_vldata_payload sz f p i))
-= (* eta expansion needed because of `weaken` *)
-  fun input len ->
-    Classical.forall_intro f_lemma;
-    validate32_fldata v (U32.v i) (Cast.uint32_to_int32 i) input len
+: Tot (validator (parse_vldata_payload sz f p i))
+= validate_weaken (parse_vldata_payload_kind sz) (validate_fldata v (U32.v i) i) ()
 
 inline_for_extraction
-let validate32_vldata_gen
+let validate_vldata_gen
+  [| validator_cls |]
   (sz: integer_size)
-  (sz32: I32.t { I32.v sz32 == sz } )
+  (sz32: U32.t { U32.v sz32 == sz } )
   (f: ((x: bounded_integer sz) -> GTot bool))
-  (f_lemma: ((x: bounded_integer sz) -> Lemma (f x == true ==> U32.v x < 2147483648)))
   (f' : ((x: bounded_integer sz) -> Tot (y: bool { y == f x })))
   (#k: parser_kind)
   (#t: Type0)
   (#p: parser k t)
-  (v32: validator32 p)
-: Tot (validator32 (parse_vldata_gen sz f p))
+  (v: validator p)
+: Tot (validator (parse_vldata_gen sz f p))
 = parse_fldata_and_then_cases_injective sz f p;
   parse_vldata_gen_kind_correct sz;
-  validate32_filter_and_then
-    (validate32_bounded_integer sz sz32)
-    (parse32_bounded_integer sz)
+  validate_filter_and_then
+    (validate_bounded_integer sz sz32)
+    (read_bounded_integer sz)
     f
     f'
     #_ #_ #(parse_vldata_payload sz f p)
-    (validate32_vldata_payload sz f f_lemma v32)
+    (validate_vldata_payload sz f v)
     ()
 
-#set-options "--z3rlimit 32"
-
 inline_for_extraction
-let validate32_bounded_vldata
+let validate_bounded_vldata
+  [| validator_cls |]
   (min: nat)
   (min32: U32.t)
   (max: nat)
@@ -79,22 +72,28 @@ let validate32_bounded_vldata
   (#k: parser_kind)
   (#t: Type0)
   (#p: parser k t)
-  (v: validator32 p)
-  (sz32: I32.t)
+  (v: validator p)
+  (sz32: U32.t)
   (u: unit {
     U32.v min32 == min /\
     U32.v max32 == max /\
-    min <= max /\ max > 0 /\ max < 2147483648 /\
-    I32.v sz32 == log256' max
+    min <= max /\
+    max > 0 /\
+    U32.v sz32 == log256' max
   })
-: Tot (validator32 (parse_bounded_vldata min max p))
+: Tot (validator (parse_bounded_vldata min max p))
 = [@inline_let]
   let sz : integer_size = log256' max in
-  fun input len ->
-    validate32_vldata_gen sz sz32 (in_bounds min max) (fun _ -> ()) (fun i -> not (U32.lt i min32 || U32.lt max32 i)) v input len
+  [@inline_let]
+  let _ = parse_bounded_vldata_correct min max p in
+  validate_strengthen
+    (parse_bounded_vldata_kind min max)
+    (validate_vldata_gen sz sz32 (in_bounds min max) (fun i -> not (U32.lt i min32 || U32.lt max32 i)) v)
+    ()
 
 inline_for_extraction
-let validate32_bounded_vldata_strong
+let validate_bounded_vldata_strong
+  [| validator_cls |]
   (min: nat)
   (min32: U32.t)
   (max: nat)
@@ -103,18 +102,24 @@ let validate32_bounded_vldata_strong
   (#t: Type0)
   (#p: parser k t)
   (s: serializer p)
-  (v: validator32 p)
-  (sz32: I32.t)
+  (v: validator p)
+  (sz32: U32.t)
   (u: unit {
     U32.v min32 == min /\
     U32.v max32 == max /\
     min <= max /\ max > 0 /\ max < 2147483648 /\
-    I32.v sz32 == log256' max
+    U32.v sz32 == log256' max
   })
-: Tot (validator32 (parse_bounded_vldata_strong min max s))
-= fun input len ->
-  validate32_bounded_vldata min min32 max max32 v sz32 () input len
+: Tot (validator (parse_bounded_vldata_strong min max s))
+= fun input pos ->
+  let h = HST.get () in
+  [@inline_let]
+  let _ = valid_facts (parse_bounded_vldata_strong min max s) h input pos in
+  [@inline_let]
+  let _ = valid_facts (parse_bounded_vldata min max p) h input pos in
+  validate_bounded_vldata min min32 max max32 v sz32 () input pos
 
+(*
 #set-options "--z3rlimit 64"
 
 inline_for_extraction
@@ -135,7 +140,7 @@ let accessor_bounded_vldata_payload
   fun input ->
   let h = HST.get () in
   parse_bounded_vldata_elim_forall min max p (B.as_seq h input);
-  let len = parse32_bounded_integer sz input in
+  let len = read_bounded_integer sz input in
   B.sub (B.offset input sz32) 0ul len
 
 inline_for_extraction
